+++
title = 'Assignment 6'
date = 2025-07-19
tags = ["MIT 18.100A"]
draft = false
+++

url: [https://ocw.mit.edu/courses/18-100a-real-analysis-fall-2020/resources/mit18_100af20_hw6/](https://ocw.mit.edu/courses/18-100a-real-analysis-fall-2020/resources/mit18_100af20_hw6/)

Chapters and exercises given with a numbering are from *Basic Analysis: Introduction to
Real Analysis (Vol I)* by J. Lebl.

### Exercise 2.5.3

Decide the convergence or divergence of the following series:

a) \(\sum_{n=1}^\infty \frac{3}{9n + 1}\)

> \(\frac{3}{9n + 1} > \frac{3}{9n + n} = \frac{3}{10n} > \frac{1}{4n}\). \(\sum_{n=1}^\infty \frac{1}{4n} = \frac{1}{4} \sum_{n=1}^\infty \frac{1}{n}\) is divergent. 
> 
> By comparison test, \(\sum_{n=1}^\infty \frac{3}{9n + 1}\) is also divergent.

b) \(\sum_{n=1}^\infty \frac{1}{2n - 1}\)

> \(\frac{1}{2n - 1} > \frac{1}{2n}\). Since \(\sum_{n=1}^\infty \frac{1}{2n}\) is divergent, \(\sum_{n=1}^\infty \frac{1}{2n - 1}\) is divergent.

c) \(\sum_{n=1}^\infty \frac{(-1)^n}{n^2}\)

> \(\left| \frac{(-1)^n}{n^2} \right| < \frac{1}{n^2}\). By the \(p\)-test, \(\sum_{n=1}^\infty \frac{1}{n^2}\) is convergent. 
> 
> Then by the comparison test, \(\sum_{n=1}^\infty \frac{(-1)^n}{n^2}\) is convergent.

d) \(\sum_{n=1}^\infty \frac{1}{n(n + 1)}\)

> \(\frac{1}{n(n + 1)} = \frac{1}{n^2 + n} < \frac{1}{n^2}\). Convergent.

e) \(\sum_{n=1}^\infty n e^{-n^2}\)

> \(n e^{-n^2} = \frac{n}{e^{n^2}} < \frac{n}{1 + n^2} < \frac{n^2}{1 + n^2} \to 1\). Convergent.


### Exercise 2.5.4

a) Prove that if \(\sum_{n=1}^\infty x_n\) converges, then \(\sum_{n=1}^\infty (x_{2n} + x_{2n+1})\) also converges.

> Let \(S_m := \sum_{n=1}^m (x_{2n} + x_{2n+1}) = \sum_{n=2}^{2m+1} x_n\). And \(s_m := \sum_{n=1}^m x_n\) is the partial sum of \(\sum x_n\).
>
> Since \(\sum x_n\) converges, \(\lim_{m \to \infty} \sum_{n=1}^m x_n = \lim_{m \to \infty} s_m = x\)
>
> Thus, \(\lim_{m \to \infty} S_m = \lim_{m \to \infty} s_{2m+1} - x_1 = x - x_1\)

b) Find an explicit example where the converse does not hold.

> Show that when \(\sum_{n=1}^\infty (x_{2n} + x_{2n+1})\) converges, \(\sum x_n\) diverges.
>
> Let \(x_n := (-1)^n\). Then \(x_{2n} + x_{2n+1} = 1 - 1 = 0\). Thus, \(\sum_{n=1}^\infty 0 = 0\) converges. But \(\sum_{n=1}^\infty x_n = \sum_{n=1}^\infty (-1)^n\) does not converge.

### Exercise 2.5.10

Prove the triangle inequality for series: If \(\sum_{n=1}^\infty x_n\) converges absolutely, then

\[
\left| \sum_{n=1}^\infty x_n \right| \leq \sum_{n=1}^\infty |x_n|.
\]

> **Claim**: For all \(m \in \mathbb{N}\), \(\left| \sum_{n=1}^m x_n \right| \leq \sum_{n=1}^m |x_n|\).
>
> **Proof**: (i) For \(m = 1\), \(|x_1| \leq |x_1|\) is trivially true.
>
> (ii) Assume the inequality holds for \(m = k\), i.e. \(\left| \sum_{n=1}^k x_n \right| \leq \sum_{n=1}^k |x_n|\). Then for \(m = k + 1\),
> \[\left| \sum_{n=1}^{k+1} x_n \right| = \left| \sum_{n=1}^k x_n + x_{k+1} \right| \leq \left| \sum_{n=1}^k x_n \right| + |x_{k+1}| \leq \sum_{n=1}^{k+1} |x_n|\]
>
> Thus by induction, \(\left| \sum_{n=1}^m x_n \right| \leq \sum_{n=1}^m |x_n|\) for all \(m \in \mathbb{N}\). \(\quad\square\)
>
> Since \(\sum_{n=1}^\infty x_n\) converges absolutely, \(\lim_{m \to \infty} \sum_{n=1}^m |x_n|\) exists. By comparison test, \(\left| \sum_{n=1}^m x_n \right|\) also converges. Taking limits from both sides: \(\left| \sum_{n=1}^\infty x_n \right| \leq \sum_{n=1}^\infty |x_n|\).

### Exercise 2.6.1

Decide the convergence or divergence of the following series:

a) \(\sum_{n=1}^\infty \frac{1}{2^{2n+1}}\)

> Let \(a_n := \frac{1}{2^{2n+1}}\). Then \(\left| \frac{a_{n+1}}{a_n} \right| = \left| \frac{2^{2n+1}}{2^{2(n+1)+1}} \right| = \frac{1}{4} < 1\). By the ratio test, \(\sum a_n\) converges absolutely.

b) \(\sum_{n=1}^\infty \frac{(-1)^n(n - 1)}{n}\)

> Let \(b_n := \frac{(-1)^n(n - 1)}{n}\). Then \(\left| \frac{b_{n+1}}{b_n} \right| = \left| -\frac{n}{n+1} \cdot \frac{n}{n - 1} \right| = \frac{n^2}{n^2 - 1} \to 1\). Ratio test does not work.
>
> Notice that \(\sum b_n\) converges if and only if \(\lim_{n \to \infty} b_n = 0\). But \(b_{2n} = \frac{2n - 1}{2n} \to 1\), and \(b_{2n - 1} = -\frac{2n - 2}{2n - 1} \to -1\). Thus \(b_n\) does not converge to 0. Therefore, \(\sum b_n\) is divergent.

c) \(\sum_{n=1}^\infty \frac{(-1)^n}{n^{1/10}}\)

> Let \(c_n := \frac{(-1)^n}{n^{1/10}}\). Since \(\frac{1}{n^{1/10}} > 0\) and is decreasing, by the alternating series test, \(\sum c_n\) converges.

d) \(\sum_{n=1}^\infty \frac{n^n}{(n + 1)^{2n}}\)

> Let \(d_n := \frac{n^n}{(n + 1)^{2n}}\). Consider \(\sup \{ |d_k|^{1/k} : k \geq n \} = \sup \left\{ \frac{k}{(k + 1)^2} : k \geq n \right\}\)
>
> Since \(0 < \frac{k}{(k + 1)^2} = \frac{1}{k + 1 + \frac{1}{k}} \leq \frac{1}{4}\), \(\frac{k}{(k + 1)^2}\) is bounded. And \(\left( \frac{k}{(k + 1)^2} \right)' = \frac{1 - k}{(1 + k)^3} < 0\) for all \(k \in (1, +\infty)\), so \(\frac{k}{(k + 1)^2}\) is monotonically decreasing, hence convergent. Therefore,  
> \[\limsup_{n \to \infty} |d_n|^{1/n} = \limsup_{n \to \infty} \sup \{ |d_k|^{1/k} : k \geq n \} = \lim_{n \to \infty} |d_n|^{1/n} = \lim_{n \to \infty} \frac{n}{(n + 1)^2} = 0 < 1\]
>
> By the root test, \(\sum d_n\) is convergent.

### Exercise 2.6.13

Find a series \(\sum_{n=1}^\infty x_n\) that converges, but \(\sum_{n=1}^\infty x_n^2\) diverges.

> Let \(x_n := \frac{(-1)^n}{\sqrt{n}}\). Since \(\lim_{n \to \infty} x_n = 0\), the series \(\sum_{n=1}^\infty x_n\) is convergent by the alternating series test.
>
> But \(\sum_{n=1}^\infty x_n^2 = \sum_{n=1}^\infty \frac{1}{n}\), which is the harmonic series and diverges.
